src/S4/vanilla.lean
@@ -1,0 +1,151 @@
+import .rules
+
+open psum nnf
+
+set_option eqn_compiler.zeta true
+
+def tableau : Π Γ : sseqt, node Γ
+| Γ := 
+match get_contra_seqt Γ with 
+| inl w := contra_rule_seqt w.2
+| inr no_contra :=
+  match get_and_seqt Γ with
+  | inl w := 
+  let inst := and_instance_seqt.cons w.2 in
+  have h : prod.measure_lex' sseqt_size (and_child Γ w.2) Γ,
+  begin apply split_lt_and_seqt end,
+  let d_delta := tableau (and_child Γ w.2) in
+  and_rule_seqt inst d_delta
+  | inr no_and := 
+    match get_or_seqt Γ with
+    | inl w := 
+    let inst := or_instance_seqt.cons w.2 in 
+    have h₁ : prod.measure_lex' sseqt_size (or_child_left Γ w.2) Γ,
+    begin apply split_lt_or_seqt_left end,
+    have h₂ : prod.measure_lex' sseqt_size (or_child_right Γ w.2) Γ,
+    begin apply split_lt_or_seqt_right end,
+    let Γ₁ := tableau (or_child_left Γ w.2) in
+    let Γ₂ := tableau (or_child_right Γ w.2) in
+    or_rule_seqt inst Γ₁ Γ₂
+    | inr no_or := 
+      match get_box_seqt Γ with
+      | inl w := -- term mode here helps termination 
+      if hb : box w.1 ∈ Γ.b then
+      let inst := box_dup_instance_seqt.cons w.2 hb in 
+      have h : prod.measure_lex' sseqt_size (box_child Γ w.2) Γ,
+      from copy_lt_seqt _ _,
+      let d_delta := tableau (box_child Γ w.2) in
+      box_rule_seqt inst d_delta
+      else 
+      let inst := box_new_instance_seqt.cons w.2 hb in 
+      have h : prod.measure_lex' sseqt_size (box_child_new Γ w.2 hb) Γ,
+      from box_new_lt_seqt _ _ _,
+      let d_delta := tableau (box_child_new Γ w.2 hb) in
+      box_new_rule_seqt inst d_delta
+      | inr no_box :=  --model.cons [] [] [] none []
+        match get_dia_seqt Γ with
+        | inl w := 
+        let ma : modal_applicable Γ := 
+            {satu := {no_and := no_and, no_or := no_or},
+             no_contra_main := no_contra, 
+             no_box_main := no_box,
+             φ := w.1,
+             ex := w.2} in 
+        let l := @dia_rule_seqt (λ Δ, prod.measure_lex' sseqt_size Δ Γ) 
+                 (λ x h, tableau x) (unmodal_seqt Γ) 
+                 (unmodal_seqt_size Γ) in
+        match l with
+        | inl w := begin left, exact unsat_of_unsat_unmodal w.1 w.2 end
+        | inr w := 
+        begin 
+        right, split, swap,
+        {let lm := models_to_tmodels w.1,
+         let sgm := dia_rule_loop Γ.h Γ.b Γ.m,
+         let mΓ : sseqt := Γ,
+         let mhtk := Γ.m,
+         have mhhtk : hintikka Γ.m, {apply hintikka_ma ma},
+         have mmhtk : Γ.m ⊆ Γ.m, {simp},
+         split, swap,
+         {let minfo : info := ⟨mΓ, mhtk, mhhtk, mmhtk⟩,
+          exact tmodel.cons minfo lm sgm },
+         {split,
+          {split,
+           {simp, intros s hs, have := list.mem_map.1 hs, 
+            rcases this with ⟨i, hmem, hi⟩, intros φ hφ, rw ←hi,
+            apply mem_be_box, exact w.2, exact hmem, exact hφ},
+           {simp, intros s hs φ hφ, exfalso, apply no_box, exact hφ},
+           {simp, intros φ hφ, 
+            by_cases hc : φ ∈ Γ.h,
+            {left, have := mem_loop_left _ Γ.b _  _ hc hφ, split, split, exact this, simp},
+            {right, have := mem_be_dia _ _ w.2 _ hφ hc, 
+             rcases this with ⟨i, hmem, hi⟩,
+             have := list.mem_map_of_mem (λ x : model, x.val) hmem,
+             split, split, exact this, exact hi} },
+           {simp, intros s rq hdesc hmem, 
+            have := ex_desc' _ _ lm _ hdesc,
+            cases this with hl hr,
+            {have hc := list.mem_map.1 hl,
+             rcases hc with ⟨ms, pmsl, pmsr⟩, 
+             have hci := be_ex _ _ w.2 _ pmsl,
+             rcases hci with ⟨iw, imem, pi⟩,
+             have ps := pt_of_m_to_tm _ _ hl,
+             have hsub := ps.1.sreq,
+             cases s with is ls sgs,
+             simp at hmem, simp at hsub,
+             have hin := hsub hmem,
+             rw pmsr at pi, simp at pi, rw pi at hin,
+             have := unmodal_sig _ _ imem _ hin,
+             cases this,
+             {right, split, swap, exact tmodel.cons is ls sgs, split, exact hdesc, simp, rw this, rw pi},
+             {left, exact this}},
+            {rcases hr with ⟨c, memc, pdc⟩, 
+             have pc := pt_of_m_to_tm _ _ memc,
+             have := pc.1.bdia, 
+             cases c with ic lc sgc, simp at this,
+             have hc := this _ _ pdc hmem,
+             cases hc with hl hr,
+             {have hcc := list.mem_map.1 memc,
+              rcases hcc with ⟨ms, pmsl, pmsr⟩, 
+              have hci := be_ex _ _ w.2 _ pmsl,
+              rcases hci with ⟨iw, imem, pi⟩,
+              have ps := pt_of_m_to_tm _ _ memc,
+              rw pmsr at pi, simp at pi, rw pi at hl,
+              have hccc := unmodal_sig _ _ imem _ hl,
+              cases hccc,
+              {right, split, swap, exact tmodel.cons ic lc sgc, split, apply tc'.base, simp, exact memc, simp, rw hccc, rw pi},
+              {left, exact hccc} },
+             {right, 
+              rcases hr with ⟨d, ddesc, hd⟩,
+              split, swap, exact d, split,
+              {apply desc_ex, split, split, exact memc, exact ddesc},
+              {exact hd}}}},
+           {simp, intros rq hrq φ hφ, cases hφ, 
+            {exfalso, apply ma.no_box_main, exact hφ}, 
+            {have := mem_loop_box _ _ _ _ hrq, rw this, exact hφ}},
+           {simp, intros s hs, have := mem_loop_dia _ _ _ _ hs, 
+            rcases this with ⟨w, hmem, hw⟩,
+            have := Γ.ha _ hmem,
+            have sb := mem_loop_box _ _ _ _ hs,
+            cases s, rw ←hw at this, rw ←sb at this, simp at this, exact this}},
+          {intros d hd, have := ex_desc' _ _ _ _ hd, 
+           cases this, 
+           {have pd := pt_of_m_to_tm _ _ this, exact pd.1}, 
+           {rcases this with ⟨m, memm, mdesc⟩, 
+            have pd := pt_of_m_to_tm _ _ memm,
+            apply pd.2, exact mdesc}}}},
+        {simp}
+        end
+end
+        | inr no_dia := 
+        let mc : model_constructible Γ := 
+          {satu := {no_and := no_and, no_or := no_or},
+           no_box_main := no_box,
+           no_contra_main := no_contra, 
+           no_dia := no_dia} in build_model mc
+        end 
+      end
+    end
+  end
+end
+using_well_founded {rel_tac := λ _ _, `[exact ⟨_, prod.measure_lex_wf' sseqt_size⟩], dec_tac := `[assumption]}
+
